Don't index expressions by their free variables.

harper/fun.v
@@ -1,18 +1,18 @@
-Require Import Sumbool String List FMapInterface Vector.
+Require Import Sumbool String List FMapInterface Vector Equality Le Lt EqNat Plus Omega.
 
 Inductive typ : Set :=
 | NumT : typ
 | StrT : typ.
 
-Inductive exp : nat -> Set :=
-| V : forall {n}, Fin.t n -> exp n
-| Num : forall {n}, nat -> exp n
-| Str : forall {n}, string -> exp n
-| Plus : forall {n}, exp n -> exp n -> exp n
-| Times : forall {n}, exp n -> exp n -> exp n
-| Cat : forall {n}, exp n -> exp n -> exp n
-| Len : forall {n}, exp n -> exp n
-| Let_ : forall {n}, exp n -> exp (S n) -> exp n.
+Inductive exp : Set :=
+| V : nat -> exp
+| Num : nat -> exp
+| Str : string -> exp
+| Plus : exp -> exp -> exp
+| Times : exp -> exp -> exp
+| Cat : exp -> exp -> exp
+| Len : exp -> exp
+| Let_ : exp -> exp -> exp.
 Notation "e1 + e2" := (Plus e1 e2)
   (at level 50, left associativity).
 Notation "e1 * e2" := (Times e1 e2)
@@ -22,19 +22,9 @@ Notation "s1 ^ s2" := (Cat s1 s2)
 
 Definition ctx := Vector.t typ.
 
-Fixpoint plusNat {n} (m : nat) (x : Fin.t n) : Fin.t (m + n) :=
-  match m as m return Fin.t (m + n) with
-    | O => x
-    | S m' => Fin.FS (plusNat m' x)
-  end.
-
 Reserved Notation "G |- e @ t" (at level 60, no associativity).
-Inductive wtexp : forall {n}, ctx n -> exp n -> typ -> Prop :=
-| OkVar : forall n (G : ctx n) (x : Fin.t n), G |- V x @ nth G x
-(*
-| OkWeaken : forall m (G' : ctx m) n (G : ctx n) (x : Fin.t n),
-  Vector.append G' G |- V (plusNat m x) @ nth G x
-*)
+Inductive wtexp : forall {n}, ctx n -> exp -> typ -> Prop :=
+| OkVar : forall n (G : ctx n) (x : nat) (xLn : x < n), G |- V x @ nth_order G xLn
 | OkStr : forall n (G : ctx n) s, G |- Str s @ StrT
 | OkNum : forall n (G : ctx n) c, G |- Num c @ NumT
 | OkPlus : forall n (G : ctx n) e1 e2,
@@ -48,15 +38,15 @@ Inductive wtexp : forall {n}, ctx n -> exp n -> typ -> Prop :=
   G |- e1 @ t1 -> Vector.cons _ t1 _ G |- e2 @ t2 -> G |- Let_ e1 e2 @ t2
 where "G |- e @ t" := (wtexp G e t).
 
-Require Import Equality.
-
-Lemma nth_append_skip : forall {elt n m} (xs : Vector.t elt n) (ys : Vector.t elt m) x,
-  nth (Vector.append xs ys) (plusNat n x) = nth ys x.
+(*
+Lemma nth_append_skip : forall {elt n m} (xs : Vector.t elt n) (ys : Vector.t elt m) xLm,
+  nth_order (Vector.append xs ys) (n + x) = nth_order ys xLm.
 Proof.
   intros elt n m xs ys x.
   induction x; induction n; dependent destruction xs; simpl; try reflexivity; apply IHn.
     intro; apply IHx.
 Qed.
+*)
 
 (*
 Lemma weaken_inv : forall {m} {G' : ctx m} {n} {G : ctx n} {x t},
@@ -84,26 +74,50 @@ Proof.
 Qed.
 *)
 
-Lemma typing_unicity : forall n (G : ctx n) (e : exp n) t,
+Lemma of_nat_lt_irr :
+  forall n m (nLm1 nLm2 : n < m), Fin.of_nat_lt nLm1 = Fin.of_nat_lt nLm2.
+Proof.
+  induction n; intros m nLm1 nLm2; destruct m.
+    inversion nLm1.
+    reflexivity.
+    inversion nLm1.
+    unfold Fin.of_nat_lt.
+    f_equal.
+    apply IHn.
+Qed.
+
+Lemma nth_order_order_irr :
+  forall {e} n (G : Vector.t e n) x (xLn : x < n) y (yLn : y < n),
+    x = y -> nth_order G xLn = nth_order G yLn.
+Proof.
+  intros e n G x xLn y yLn xEy.
+  destruct xEy.
+  unfold nth_order, Fin.of_nat_lt.
+  f_equal.
+  apply of_nat_lt_irr.
+Qed.
+
+Lemma typing_unicity : forall n (G : ctx n) (e : exp) t,
   G |- e @ t -> forall t', G |- e @ t' -> t = t'.
 Proof.
   intros n G e t oke t' oke'.
   dependent induction oke; dependent destruction oke'; try reflexivity.
-  cut (t1 = t0).
-    destruct 1; apply IHoke2; assumption.
-    apply IHoke1; assumption.
+    apply nth_order_order_irr; reflexivity.
+    cut (t1 = t0).
+      destruct 1; apply IHoke2; assumption.
+      apply IHoke1; assumption.
 Qed.
 
-Fixpoint esuc {n} (e : exp n) : exp (S n) :=
+Fixpoint esuc (e : exp) : exp :=
   match e with
-    | V _ x => V (Fin.FS x)
-    | Num _ c => Num c
-    | Str _ s => Str s
+    | V x => V (1 + x)
+    | Num c => Num c
+    | Str s => Str s
     | c1 + c2 => esuc c1 + esuc c2
     | c1 * c2 => esuc c1 * esuc c2
     | s1 ^ s2 => esuc s1 ^ esuc s2
-    | Len _ e1 => Len (esuc e1)
-    | Let_ _ e1 e2 => Let_ (esuc e1) (esuc e2)
+    | Len e1 => Len (esuc e1)
+    | Let_ e1 e2 => Let_ (esuc e1) (esuc e2)
   end.
 
 Fixpoint dist (n m : nat) :=
@@ -113,131 +127,193 @@ Fixpoint dist (n m : nat) :=
     | S n', S m' => dist n' m'
   end.
 
-Fixpoint eswapn {n} (m : nat) (e : exp (S (S n))) : exp (S (S n)) :=
-  match e in exp n' return n' = S (S n) -> S (S n) = n' -> exp n' with
-    | V _ x => fun eqN eqNr =>
-      match dist (projT1 (Fin.to_nat x)) m with
-        | O => eq_rect _ exp (V (Fin.FS Fin.F1)) _ eqNr
-        | S O => eq_rect _ exp (V Fin.F1) _ eqNr
-        | S (S x') => V x
-      end
-    | Num _ c => fun _ _ => Num c
-    | Str _ s => fun _ _ => Str s
-    | e1 + e2 => fun eqN eqNr =>
-      eq_rect
-        _ exp
-        (eswapn m (eq_rect _ exp e1 _ eqN) + eswapn m (eq_rect _ exp e2 _ eqN))
-        _ eqNr
-    | e1 * e2 => fun eqN eqNr =>
-      eq_rect
-        _ exp
-        (eswapn m (eq_rect _ exp e1 _ eqN) * eswapn m (eq_rect _ exp e2 _ eqN))
-        _ eqNr
-    | s1 ^ s2 => fun eqN eqNr =>
-      eq_rect
-        _ exp
-        (eswapn m (eq_rect _ exp s1 _ eqN) ^ eswapn m (eq_rect _ exp s2 _ eqN))
-        _ eqNr
-    | Len _ e1 => fun eqN eqNr =>
-      eq_rect
-        _ exp
-        (Len (eswapn m (eq_rect _ exp e1 _ eqN)))
-        _ eqNr
-    | Let_ _ e1 e2 => fun eqN eqNr =>
-      eq_rect
-        _ exp
-        (Let_ (eswapn m (eq_rect _ exp e1 _ eqN))
-              (eswapn (S m) (eq_rect _ (fun n => exp (S n)) e2 _ eqN)))
-        _ eqNr
-  end eq_refl eq_refl.
 (*
-  refine (
-    let P (n : nat) (e : exp n) : Set :=
-          match n with
-            | O => unit
-            | S O => unit
-            | S (S n') => exp (S (S n'))
-          end
-    in exp_rec
-         P
-         (fun n x => match dist (projT1 (Fin.to_nat x)) m with
-                       | O => _
-                       | S O => _
-                       | S (S x') => _
-                     end)
-         (fun n c => _)
-         (fun n s => _)
-         (fun n e1 e1' e2 e2' => _) (*e1' + e2'*)
-         (fun n e1 e1' e2 e2' => _) (*e1' * e2'*)
-         (fun n s1 s1' s2 s2' => _) (*s1' ^ s2'*)
-         (fun n e1 e1' => _)
-         (fun n e1 e1' e2 e2' => _)
-         (S (S n)) e); destruct n0; try exact tt; try (destruct n0; try exact tt).
-  simpl; exact (V (Fin.FS Fin.F1)).
-  simpl; exact (V Fin.F1).
-  simpl. exact (V (Fin.FS (Fin.FS x))).
-  exact (Num c).
-  exact (Str s).
-  exact (e1' + e2').
-  exact (e1' * e2').
-  exact (s1' ^ s2').
-  exact (Len e1').
-  exact (Let_ e1' e2').
-Defined.
+    m
+Gl, t1, t2, Gr
+==> |Gl| = m
+==> x = m   => S x
+    x = S m => x
 *)
-Definition eswap {n} (e : exp (S (S n))) : exp (S (S n)) := eswapn 0 e.
 
-Fixpoint eswapn' {n} (m : nat) (okn : 2 <= n) (e : exp n) : exp n :=
+Fixpoint eswapn (m : nat) (e : exp) : exp :=
   match e with
-    | V _ x => fun eqN eqNr =>
-      match dist (projT1 (Fin.to_nat x)) m with
-        | O => eq_rect _ exp (V (Fin.FS Fin.F1)) _ eqNr
-        | S O => eq_rect _ exp (V Fin.F1) _ eqNr
-        | S (S x') => V x
-      end
+    | V x =>
+      if beq_nat x m then V (S m)
+        else if beq_nat x (S m) then V m
+          else V x
+    | Num c => Num c
+    | Str s => Str s
+    | e1 + e2 => eswapn m e1 + eswapn m e2
+    | e1 * e2 => eswapn m e1 * eswapn m e2
+    | s1 ^ s2 => eswapn m s1 ^ eswapn m s2
+    | Len e1 => Len (eswapn m e1)
+    | Let_ e1 e2 => Let_ (eswapn m e1) (eswapn (S m) e2)
   end.
-  
+Definition eswap (e : exp) : exp := eswapn 0 e.
 
-Lemma exchange : forall n (Gl : ctx n) m (Gr : ctx m) (e : exp (n + S (S m))) t t1 t2,
+Lemma cons_append_comm : forall {e} x {n} (xs : Vector.t e n) {m} (ys : Vector.t e m),
+  Vector.cons _ x _ (Vector.append xs ys) = Vector.append (Vector.cons _ x _ xs) ys.
+Proof.
+  intros e x n xs m ys.
+  induction xs; simpl; reflexivity.
+Qed.
+
+Lemma eq_to_JMeq : forall A (x y : A), x = y -> x ~= y.
+Proof.
+  intros A x y xEy; rewrite xEy; reflexivity.
+Qed.
+
+Lemma strengthen_var : forall n (G : ctx n) x t t1,
+  cons _ t1 _ G |- V (S x) @ t -> G |- V x @ t.
+Proof.
+  intros n G x t t1 okv.
+  dependent destruction okv.
+    unfold nth_order, nth.
+    apply OkVar.
+Qed.
+
+Lemma nth_order_cons :
+  forall {e n} (x : e) (xs : Vector.t e n) y (yLn : y < n) (SyLSn : S y < S n),
+    nth_order xs yLn = nth_order (cons _ x _ xs) SyLSn.
+Proof.
+  intros e n x xs y yLn SyLSn.
+  destruct y; destruct n.
+    inversion yLn.
+    reflexivity.
+    inversion yLn.
+    unfold nth_order, nth.
+    simpl.
+    f_equal.
+    f_equal.
+    apply of_nat_lt_irr.
+Qed.
+
+(* FIXME *)
+Lemma nth_order_append :
+  forall {e n} (ws : Vector.t e n) {m} (xs : Vector.t e m)
+         y (yLm : y < m) z (zEp : z = y + n) (zL : z < n + m),
+    nth_order xs yLm = nth_order (append ws xs) zL.
+Proof.
+  intros e n ws m xs y yLm z zL.
+  induction ws.
+    simpl; apply (nth_order_order_irr _ xs y yLm _ zL).
+      rewrite plus_comm; reflexivity.
+    rewrite <- cons_append_comm.
+    rewrite (nth_order_cons ).
+Qed.
+
+Lemma weaken_var : forall n (G : ctx n) x t t1,
+  G |- V x @ t -> cons _ t1 _ G |- V (S x) @ t.
+Proof.
+  intros n G x t t1 okv.
+  dependent destruction okv.
+    rewrite (nth_order_cons t1 _ _ _ (lt_n_S _ _ xLn)).
+    apply OkVar.
+Qed.
+
+Lemma exchange : forall n (Gl : ctx n) m (Gr : ctx m) (e : exp) t t1 t2,
   Vector.append Gl (Vector.cons _ t1 _ (Vector.cons _ t2 _ Gr)) |- e @ t ->
-  Vector.append Gl (Vector.cons _ t2 _ (Vector.cons _ t1 _ Gr)) |- eswap e @ t.
+  Vector.append Gl (Vector.cons _ t2 _ (Vector.cons _ t1 _ Gr)) |- eswapn (S n) e @ t.
 Proof.
-
-Lemma exchange : forall n (G : ctx n) (e : exp (S (S n))) t t1 t2,
-  Vector.cons _ t1 _ (Vector.cons _ t2 _ G) |- e @ t ->
-  Vector.cons _ t2 _ (Vector.cons _ t1 _ G) |- eswap e @ t.
-Proof.
-  intros n G e t t1 t2 oke.
+  intros n Gl m Gr e t t1 t2 oke.
   dependent induction oke.
-    unfold eswap, eswapn; simpl.
-      dependent destruction x.
+  unfold eswapn.
+  remember (beq_nat x (S n)).
+  destruct b.
+    assert (S n = x) by admit.
+    destruct H.
+    unfold nth_order, nth.
+    simpl.
+    
+    
+
+  induction n.
+    destruct x.
+      dependent destruction Gl.
+      refine (OkVar _ (cons _ t2 _ (cons _ t1 _ Gr)) 1 _); apply lt_n_S; apply lt_0_Sn.
+      destruct x.
+        dependent destruction Gl.
+        refine (OkVar _ (cons _ t2 _ (cons _ t1 _ Gr)) 0 _); apply lt_0_Sn.
+        dependent destruction Gl.
+        simpl in xLn.
+        rewrite <- (nth_order_cons t1 (cons _ t2 _ Gr) _ (lt_S_n _ _ xLn) _).
+        rewrite <- (nth_order_cons t2 Gr _ (lt_S_n _ _ (lt_S_n _ _ xLn)) _).
+        apply weaken_var.
+        apply weaken_var.
+        apply OkVar.
+    destruct x.
+      destruct n.
+      dependent destruction Gl.
+      simpl.
+      unfold nth_order, nth.
+      simpl.
+      assert (h = nth_order (cons typ h (S (S m)) (append Gl (cons typ t2 (S m) (cons typ t1 m Gr)))) xLn).
+        unfold nth_order, nth.
+        reflexivity.
+      rewrite H.
       apply OkVar.
-      dependent destruction x.
+      simpl.
+      dependent destruction Gl.
+      unfold nth_order, nth.
+      simpl.
+      assert (h = nth_order (cons typ h (S (n + S (S m)))
+                              (append Gl (cons typ t2 (S m) (cons typ t1 m Gr)))) xLn).
+        unfold nth_order, nth.
+        reflexivity.
+      rewrite H.
       apply OkVar.
 
-      (* FIXME *)
-      assert (exists n', S (S n') = dist (projT1 (Fin.to_nat (Fin.FS (Fin.FS x)))) 0)
-        by admit.
-      destruct H.
-      rewrite <- H.
+
+
+      
+
+  destruct x.
+    destruct n.
+      dependent destruction Gl.
       simpl.
-      cut (nth (cons typ t2 (S n) (cons typ t1 n G)) (Fin.FS (Fin.FS x)) = nth G x).
-        intro.
-        rewrite <- H0.
+      refine (OkVar (S (S m)) (cons _ t2 _ (cons _ t1 _ Gr)) 1 _).
+      apply le_n_S; apply le_n_S; apply le_0_n.
+        destruct n; dependent destruction Gl.
+          refine (OkVar _ (append (cons _ h _ Gl) (cons _ t2 _ (cons _ t1 _ Gr))) 0 _).
+            apply le_n_S; apply le_0_n.
+          refine (OkVar _ (append (cons _ h _ Gl) (cons _ t2 _ (cons _ t1 _ Gr))) 0 _).
+            apply le_n_S; apply le_0_n.
+      destruct n.
+        dependent destruction Gl.
+        destruct x.
+          refine (OkVar _ (cons _ t2 _ (cons _ t1 _ Gr)) 0 _).
+            apply le_n_S; apply le_0_n.
+          simpl.
+          simpl in xLn.
+          rewrite <- (nth_order_cons t1 (cons _ t2 _ Gr) _ (lt_S_n _ _ xLn) _).
+          rewrite <- (nth_order_cons t2 Gr _ (lt_S_n _ _ (lt_S_n _ _ xLn)) _).
+          apply weaken_var.
+          apply weaken_var.
+          apply OkVar.
+          simpl.
+          dependent destruction Gl.
+          destruct (dist x n).
+ 
+        
+| OkVar : forall n (G : ctx n) (x : nat) (xLn : x < n), G |- V x @ nth_order G xLn
+        unfold nth_order, nth.
+        simpl.
         apply OkVar.
-        apply (nth_append_skip (Vector.cons _ t2 _ (Vector.cons _ t1 _ (Vector.nil _)))
-                               G x).
-      apply OkStr.
-      apply OkNum.
-      apply OkPlus; [apply IHoke1 | apply IHoke2]; reflexivity.
-      apply OkTimes; [apply IHoke1 | apply IHoke2]; reflexivity.
-      apply OkCat; [apply IHoke1 | apply IHoke2]; reflexivity.
-      apply OkLen; apply IHoke; reflexivity.
-      apply (OkLet _ _ _ t0).
-        apply IHoke1; reflexivity.
-        fold (eswapn (n:=S n)).
-        apply (IHoke2 _ (Vector.cons _ t1 _ G) _ t2 t0). reflexivity.
-| OkLet : forall n (G : ctx n) e1 t1 e2 t2,
+
+    apply OkStr.
+    apply OkNum.
+    apply OkPlus; [apply IHoke1 | apply IHoke2]; reflexivity.
+    apply OkTimes; [apply IHoke1 | apply IHoke2]; reflexivity.
+    apply OkCat; [apply IHoke1 | apply IHoke2]; reflexivity.
+    apply OkLen; apply IHoke; reflexivity.
+    unfold eswap, eswapn.
+    fold eswapn.
+    apply (OkLet _ _ (eswapn n e1) t0 (eswapn (S n) e2)).
+      apply IHoke1; reflexivity.
+      rewrite cons_append_comm.
+      apply (IHoke2 (S n) (cons _ t0 _ Gl) _ Gr t1 t2).
+        reflexivity.
+        apply eq_to_JMeq; apply cons_append_comm.
 Qed.
 
 Lemma weakening : forall n (G : ctx n) (e : exp n) t,
